test/general/test_union.c
@@ -4,9 +4,15 @@
 #include "../include/PulseMacros.h"
 
 
+// struct abcd {
+//          unsigned int a;
+//          bool b;
+//          uint8_t c[10];
+// };
+
 union ab {
-         unsigned int a;
-         bool b;
+  unsigned int a;
+  bool b;      
 };
 
 ERASED_ARG(s:_)
@@ -15,9 +21,18 @@ REQUIRES(ab_pred x s)
 REQUIRES(pure (UInt32.fits (UInt32.v (Case_ab_a?._0 s) + 1)))
 ENSURES(exists* s'. ab_pred x s')
 void incr_a(union ab *x) {
+  LEMMA(ab_is_a (!x));
   LEMMA(ab_explode !x);
-  LEMMA(rewrite each s as Case_ab_a (Case_ab_a?._0 s));
   x->a = x->a + 1;
+  LEMMA(ab_recover !x #(Case_ab_a _));
+}
+
+REQUIRES(exists* s. ab_pred x s)
+ENSURES(ab_pred x (Case_ab_a v))
+void set_case_a(union ab *x, unsigned int v) {
+  LEMMA(ab_change_a !x);
+  LEMMA(ab_explode !x);
+  x->a = v;
   LEMMA(ab_recover !x #(Case_ab_a _));
 }
 
@@ -27,39 +42,36 @@ struct stru {
 };
 
 INCLUDE(
-"let stru_ok (u : ref stru) (s : stru_spec) : slprop =\
-stru_pred u s **\
-pure (\
-match s.tag with\
-| 0y -> Case_ab_a? s.payload\
-| 1y -> Case_ab_b? s.payload\
-| _ -> false\
-)"
+[@@pulse_unfold]
+let stru_ok (u : ref stru) (s : stru_spec) : slprop =
+stru_pred u s **
+pure (
+match s.tag with
+| 0y -> Case_ab_a? s.payload
+| 1y -> Case_ab_b? s.payload
+| _ -> False
+)
 )
 
 
-
-EXPECT_FAILURE()
-ERASED_ARG(#s : stru_spec)
-REQUIRES(stru_pred foo s)
-ERASED_ARG(s:_)
-REQUIRES(pure (Case_ab_a? s))
-REQUIRES(ab_pred foo.payload s)
-REQUIRES(pure (UInt32.fits (UInt32.v (Case_ab_a?._0 s) + 1)))
-ENSURES(exists* s'. ab_pred foo.payload s')
-ENSURES("exists* (s':stru_spec). stru_pred foo s' ** pure (s' == {tag = s.tag; payload = s.payload})")
+PRESERVES(exists* s. stru_ok foo s)
 void test_union(struct stru * foo){
-
+  LEMMA(stru_explode (!foo));
   if (foo->tag == 0){
-    foo->payload.a += 1; 
+    LEMMA(ab_is_a (! (! foo)).payload);
+    LEMMA(ab_explode (! (!foo)).payload);
+    foo->payload.a = 1;
+    LEMMA(ab_recover (! (!foo)).payload #(Case_ab_a _));
+    LEMMA(stru_recover (!foo));
   }
-  else if (foo->tag == 1){
-    foo->payload.b = !(foo->payload.b);
+  else if (foo->tag == 1) {
+    LEMMA(ab_is_b (! (! foo)).payload);
+    LEMMA(ab_explode (! (!foo)).payload);
+    foo->payload.b = false;
+    LEMMA(ab_recover (! (!foo)).payload #(Case_ab_b _));
+    LEMMA(stru_recover (!foo));    
+  }
+  else {
+    LEMMA(unreachable());
   }
 }
-
-
-
-
-
-
